

Algorithm derivation through Flame

Victor Eijkhout, Susan Lindsey

Fall 2025

last formatted: October 30, 2025

Dijkstra quote, part 1

Today a usual technique is to make a program and then to test it. But: program testing can be a very effective way to show the presence of bugs, but is hopelessly inadequate for showing their absence. (cue laughter)

Dijkstra quote, part 2

The only effective way to raise the confidence level of a program significantly is to give a convincing proof of its correctness. But one should not first make the program and then prove its correctness, because then the requirement of providing the proof would only increase the poor programmer's burden. On the contrary: the programmer should let correctness proof and program grow hand in hand.

Matrix-vector product

$$y = Ax$$

Partitioned:

$$\begin{pmatrix} y_T \\ y_B \end{pmatrix} = \begin{pmatrix} A_T \\ A_B \end{pmatrix} (x)$$

Two equations:

$$\begin{cases} y_T = A_T x \\ y_B = A_B x \end{cases}$$

Inductive construction

$$\begin{pmatrix} y_T \\ y_B \end{pmatrix} = \begin{pmatrix} A_T \\ A_B \end{pmatrix} (x)$$

Assume only equation

$$y_T = A_T x$$

is satisfied, and grow the T block by one row.

Algorithm outline

$$\begin{pmatrix} y_T \\ y_B \end{pmatrix} = \begin{pmatrix} A_T \\ A_B \end{pmatrix} (x)$$

While T is not the whole system

 Predicate: $y_T = A_T x$ true

 Update: grow T block by one

 Predicate: $y_T = A_T x$ true for new/bigger T block

Note initial and final condition.

Inductive step

Here is the big trick

Before

$$\begin{pmatrix} y_T \\ y_B \end{pmatrix} = \begin{pmatrix} A_T \\ A_B \end{pmatrix} (x)$$

split:

$$\begin{pmatrix} Y_1 \\ \dots \\ y_2 \\ Y_3 \end{pmatrix} = \begin{pmatrix} A_1 \\ \dots \\ a_2 \\ A_3 \end{pmatrix} (x)$$

Then the update step, and

After

$$\begin{pmatrix} Y_1 \\ y_2 \\ \dots \\ Y_3 \end{pmatrix} = \begin{pmatrix} A_1 \\ a_2 \\ \dots \\ A_3 \end{pmatrix} (x)$$

and unsplit

$$\begin{pmatrix} y_T \\ y_B \end{pmatrix} = \begin{pmatrix} A_T \\ A_B \end{pmatrix} (x)$$

Before the update:

$$\begin{pmatrix} Y_1 \\ \dots \\ y_2 \\ Y_3 \end{pmatrix} = \begin{pmatrix} A_1 \\ \dots \\ a_2 \\ A_3 \end{pmatrix} (x)$$

so

$$Y_1 = A_1 x$$

is true

Then the update step, and

After

$$\begin{pmatrix} Y_1 \\ y_2 \\ \dots \\ Y_3 \end{pmatrix} = \begin{pmatrix} A_1 \\ a_2 \\ \dots \\ A_3 \end{pmatrix} (x)$$

so

$$\begin{cases} Y_1 = A_1 x & \text{we had this} \\ y_2 = a_2 x & \text{we need this} \end{cases}$$

Resulting algorithm

While T is not the whole system

Predicate: $y_T = A_T x$ true

Update: $y_2 = a_2 x$

Predicate: $y_T = A_T x$ true for new/bigger T block

In traditional notation:

Do $n = 0..N - 1$

Predicate: $y_{0:n} = A_{0:n,*} x$ true

Compute: $y_n = a_{n,*} x$

Predicate: $y_{0:n+1} = A_{0:n+1,*} x$ true

So what?

We already know this stuff, right?

Well, we made an assumption on how to partition the matrix.
What if we partition it differently?

Matrix-vector product, the other way around

$$y = Ax$$

Partitioned:

$$(y) = (A_L \quad A_R) \begin{pmatrix} x_T \\ x_B \end{pmatrix}$$

Equation:

$$\left\{ y = A_L x_T + A_R x_B \right.$$

Inductive construction

$$(y) = (A_L \quad A_R) \begin{pmatrix} x_T \\ x_B \end{pmatrix}$$

Assume

$$y = A_L x_T$$

is constructed, and grow the T block.

Inductive step

Before

$$(y) = (A_L \quad A_R) \begin{pmatrix} x_T \\ x_B \end{pmatrix}$$

split:

$$(y) = \begin{pmatrix} A_1 & \vdots & A_2 & A_3 \end{pmatrix} \begin{pmatrix} x_1 \\ \dots \\ x_2 \\ x_3 \end{pmatrix}$$

Then the update step, and

After

$$(y) = \begin{pmatrix} A_1 & A_2 & \vdots & A_3 \end{pmatrix} \begin{pmatrix} x_1 \\ x_2 \\ \dots \\ x_3 \end{pmatrix}$$

and unsplit

$$(y) = (A_L \quad A_R) \begin{pmatrix} x_T \\ x_B \end{pmatrix}$$

Derivation of the update

Before the update:

$$(y) = \begin{pmatrix} A_1 & \vdots & A_2 & A_3 \end{pmatrix} \begin{pmatrix} x_1 \\ \dots \\ x_2 \\ x_3 \end{pmatrix}$$

so

$$y = A_1 x_1$$

is true

Then the update step, and

After

$$(y) = \begin{pmatrix} A_1 & A_2 & \vdots & A_3 \end{pmatrix} \begin{pmatrix} x_1 \\ x_2 \\ \dots \\ x_3 \end{pmatrix}$$

so

$$y = A_1 x_1 + A_2 x_2$$

in other words, we need

$$y \leftarrow y + A_2 x_2$$

Resulting algorithm

While T is not the whole system

Predicate: $y = A_L x_T$ true

Update: $y \leftarrow y + A_2 x_2$

Predicate: $y = A_L x_T$ true for new/bigger T block

Two algorithms

for $r = 1, m$
 $y_r = A_{r,*}x_*$

$y \leftarrow 0$
for $c = 1, n$
 $y \leftarrow y + A_{*,c}x_c$

Take it from here

This gets more interesting if you take other algorithms:

- Matrix-matrix multiplication
- Matrix inversion
- Sylvester equation
- Iterative linear system solving

<https://shpc.oden.utexas.edu/>